% SPDX-License-Identifier: CC-BY-SA-4.0
% Author: Matthieu Perrin
% Part: 
% Section: 
% Sub-section: 
% Frame: 

\begingroup


\begin{frame}{Opérations ensemblistes (1)}
  Soit $E$ un ensemble. Soient $A, B, C \in \mathscr{P}(E)$
  \begin{block}{Définition -- union et intersection}
    \begin{description}
    \item[Union :] $A \cup B \eqdef \{x \in E \,|\, x \in A \lor x \in B\}$
    \item[Intersection :] $A \cap B \eqdef \{x \in E \,|\, x \in A \land x \in B\}$
    \end{description}
  \end{block}
  \begin{block}{Propriétés}
    \begin{description}
    \item[Associativité :] \alert{$(A \cup B) \cup C = A \cup (B \cup C)$} et \alert{$(A \cap B) \cap C = A \cap (B \cap C)$}
    \item[Commutativité :] \alert{$A \cup B = B \cup A$} et \alert{$A \cap B = B \cap A$}
    \item[Idempotence :] \alert{$A \cup A = A = A \cap A$}
    \item[Neutralité :] \alert{$A \cup \emptyset = A = A \cap E$}
    \item[Absorption :] \alert{$A \cup E = E$} et \alert{$A \cap \emptyset = \emptyset$}
    \item[Distributivité :] \alert{$A \cup (B \cap C) = (A \cup B) \cap (A \cup C)$} et \alert{$A \cap (B \cup C) = (A \cap B) \cup (A \cap C)$}
    \end{description}
  \end{block}
\end{frame}
\endgroup
